implement toy eager and lazy file systems, and try to prove them correct.
the eager file system is proven correct according to the spec.

what previously seemed to be a weirdness in my new spec turns out to
be a critical problem that prevents proving the lazy file system correct.

in particular, the spec in effect requires that Sync force the last
Write to disk, even if that Write happened before a Crash.  but the
lazy file system forgets the in-memory state after a Crash, and since
it forgot the last (pre-Crash) Write, it cannot force it to disk..

Fs.v
@@ -82,7 +82,9 @@ Inductive last_wrote: history -> nat -> Prop :=
     last_wrote h n -> last_wrote (Sync :: h) n
   | last_wrote_crash:
     forall (h:history) (n:nat),
-    last_wrote h n -> last_wrote (Crash :: h) n.
+    last_wrote h n -> last_wrote (Crash :: h) n
+  | last_wrote_nil:
+    last_wrote nil 0.
 
 (* (wrote_since_sync h n) means n was either the last thing written before
    the last sync, or was written after the last sync *)
@@ -107,7 +109,9 @@ Inductive wrote_since_sync: history -> nat -> Prop :=
        across many crashes, until it's finally Sync'ed.
      *)
     forall (h:history) (n:nat),
-    wrote_since_sync h n -> wrote_since_sync (Crash :: h) n.
+    wrote_since_sync h n -> wrote_since_sync (Crash :: h) n
+  | wrote_since_sync_nil:
+    wrote_since_sync nil 0.
 
 (* (could_read h n) means n could be the return value of a read *)
 Inductive could_read: history -> nat -> Prop :=
@@ -122,7 +126,9 @@ Inductive could_read: history -> nat -> Prop :=
     could_read h n -> could_read (Sync :: h) n
   | could_read_crash:
     forall (h:history) (n:nat),
-    wrote_since_sync h n -> could_read (Crash :: h) n.
+    wrote_since_sync h n -> could_read (Crash :: h) n
+  | could_read_nil:
+    could_read nil 0.
 
 Inductive legal2: history -> Prop :=
   | legal2_read:
@@ -158,3 +164,190 @@ Theorem test_legal2_weird:
 Proof.
   repeat constructor.
 Qed.
+
+(* Toy implementations of a file system *)
+
+Inductive invocation : Set :=
+  | do_read: invocation
+  | do_write: nat -> invocation
+  | do_sync: invocation
+  | do_crash: invocation.
+
+(* Eager file system *)
+
+Definition eager_state := nat.
+
+Definition eager_init := 0.
+
+Definition eager_apply (s: eager_state) (i: invocation) : eager_state * event :=
+  match i with
+  | do_read => (s, Read s)
+  | do_write n => (n, Write n)
+  | do_sync => (s, Sync)
+  | do_crash => (s, Crash)
+  end.
+
+(* Lazy file system *)
+
+Record lazy_state : Set := mklazy {
+  LazyMem: nat;
+  LazyDisk: nat
+}.
+
+Definition lazy_init := mklazy 0 0.
+
+Definition lazy_apply (s: lazy_state) (i: invocation) : lazy_state * event :=
+  match i with
+  | do_read => (s, Read s.(LazyMem))
+  | do_write n => (mklazy n s.(LazyDisk), Write n)
+  | do_sync => (mklazy s.(LazyMem) s.(LazyMem), Sync)
+  | do_crash => (mklazy s.(LazyDisk) s.(LazyDisk), Crash)
+  end.
+
+(* What does it mean for a file system to be correct? *)
+
+Fixpoint fs_apply_list (state_type: Set)
+                       (fs_init: state_type)
+                       (fs_apply: state_type -> invocation -> state_type * event)
+                       (l: list invocation)
+                       : state_type * history :=
+  match l with
+  | i :: rest =>
+    match fs_apply_list state_type fs_init fs_apply rest with
+    | (s, h) =>
+      match fs_apply s i with
+      | (s', e) => (s', e :: h)
+      end
+    end
+  | nil => (fs_init, nil)
+  end.
+
+Definition fs_legal2 (state_type: Set)
+                     (fs_init: state_type)
+                     (fs_apply: state_type -> invocation -> state_type * event) :=
+  forall (l: list invocation) (h: history) (s: state_type),
+  fs_apply_list state_type fs_init fs_apply l = (s, h) ->
+  legal2 h.
+
+(* Eager FS is correct *)
+
+Lemma eager_last_wrote:
+  forall (l: list invocation) (s: eager_state) (h: history),
+  fs_apply_list eager_state eager_init eager_apply l = (s, h) ->
+  last_wrote h s.
+Proof.
+  induction l.
+  - crush; inversion H; unfold eager_init; constructor.
+  - destruct a; unfold fs_apply_list; fold fs_apply_list; simpl;
+    case_eq (fs_apply_list eager_state eager_init eager_apply l);
+    intros; inversion H0.
+    + constructor.  apply IHl.  crush.
+    + constructor.
+    + constructor.  apply IHl.  crush.
+    + constructor.  apply IHl.  crush.
+Qed.
+
+Lemma last_wrote_wrote_since_sync:
+  forall h n,
+  last_wrote h n -> wrote_since_sync h n.
+Proof.
+  induction h.
+  - crush.  inversion H.  constructor.
+  - destruct a; intros; inversion H.
+    + constructor.  apply IHh.  auto.
+    + constructor.
+    + constructor.  auto.
+    + constructor.  apply IHh.  auto.
+Qed.
+
+Lemma last_wrote_could_read:
+  forall h n,
+  last_wrote h n -> could_read h n.
+Proof.
+  induction h.
+  - crush.  inversion H.  constructor.
+  - destruct a; intros; inversion H.
+    + constructor.  apply IHh.  auto.
+    + constructor.
+    + constructor.  apply IHh.  auto.
+    + constructor.  apply last_wrote_wrote_since_sync.  auto.
+Qed. 
+
+Theorem eager_correct:
+  fs_legal2 eager_state eager_init eager_apply.
+Proof.
+  unfold fs_legal2.
+  induction l.
+  - crush; inversion H; constructor.
+  - destruct a; unfold fs_apply_list; fold fs_apply_list; simpl;
+    case_eq (fs_apply_list eager_state eager_init eager_apply l);
+    intros; inversion H0.
+    + constructor.
+      * apply last_wrote_could_read.  eapply eager_last_wrote.  rewrite <- H2.  exact H.
+      * apply IHl with (s:=e).  auto.
+    + constructor; apply IHl with (s:=e); crush.
+    + constructor; apply IHl with (s:=e); crush.
+    + constructor; apply IHl with (s:=e); crush.
+Qed.
+
+(* Lazy FS correct *)
+
+Inductive wrote_before_sync: history -> nat -> Prop :=
+  | wrote_before_sync_read:
+    forall (h:history) (n:nat) (rn:nat),
+    wrote_before_sync h n -> wrote_before_sync ((Read rn) :: h) n
+  | wrote_before_sync_write:
+    forall (h:history) (n:nat) (wn:nat),
+    wrote_before_sync h n -> wrote_before_sync ((Write wn) :: h) n
+  | wrote_before_sync_sync:
+    forall (h:history) (n:nat),
+    last_wrote h n -> wrote_before_sync (Sync :: h) n
+  | wrote_before_sync_crash:
+    forall (h:history) (n:nat),
+    wrote_before_sync h n -> wrote_before_sync (Crash :: h) n
+  | wrote_before_sync_nil:
+    wrote_before_sync nil 0.
+
+Lemma lazy_could_read:
+  forall (l: list invocation) (s: lazy_state) (h: history),
+  fs_apply_list lazy_state lazy_init lazy_apply l = (s, h) ->
+  could_read h (LazyMem s) /\ wrote_before_sync h (LazyDisk s).
+Proof.
+  induction l.
+  - crush; inversion H; unfold eager_init; constructor.
+  - destruct a; unfold fs_apply_list; fold fs_apply_list; simpl;
+    case_eq (fs_apply_list lazy_state lazy_init lazy_apply l);
+    intros; inversion H0.
+    + split.
+      * constructor.  apply IHl.  crush.
+      * constructor.  apply IHl.  crush.
+    + split.
+      * constructor.
+      * constructor.  simpl.  apply IHl.  crush.
+    + split.
+      * constructor.  simpl.  apply IHl.  auto.
+      * simpl.  constructor.
+        (* XXX not provable due to the weirdness illustated by test_legal2_weird:
+           according to the spec, Sync forces the last write to disk, even if that
+           last write happened before a Crash!
+         *)
+Abort.
+
+(*
+Theorem lazy_correct:
+  fs_legal2 lazy_state lazy_init lazy_apply.
+Proof.
+  unfold fs_legal2.
+  induction l.
+  - crush; inversion H; constructor.
+  - destruct a; unfold fs_apply_list; fold fs_apply_list; simpl;
+    case_eq (fs_apply_list lazy_state lazy_init lazy_apply l);
+    intros; inversion H0.
+    + constructor.
+      * apply lazy_could_read with (l:=l).  rewrite <- H2.  auto.
+      * apply IHl with (s:=l0).  auto.
+    + constructor; apply IHl with (s:=l0); crush.
+    + constructor; apply IHl with (s:=l0); crush.
+    + constructor; apply IHl with (s:=l0); crush.
+Qed.
+*)
